lib ccorres_rewrite: discard everything sequenced after a Throw
Also introduce simple conditional rewriting.

lib/clib/CCorres_Rewrite.thy
@@ -1,229 +1,48 @@
 (*
- * Copyright 2016, NICTA
+ * Copyright 2018, Data61
+ * Commonwealth Scientific and Industrial Research Organisation (CSIRO)
+ * ABN 41 687 119 230.
  *
  * This software may be distributed and modified according to the terms of
  * the BSD 2-Clause license. Note that NO WARRANTY is provided.
  * See "LICENSE_BSD2.txt" for details.
  *
- * @TAG(NICTA_BSD)
+ * @TAG(DATA61_BSD)
  *)
-
-(* This theory provides a very basic proof method for rewriting SIMPL (C) programs
-  under ccorres/ccorres_underlying using semantic equivalence.
-*)
 
 theory CCorres_Rewrite
 imports
   "Corres_UL_C"
+  "Simpl_Rewrite"
 begin
 
-(* C_simp rules may be applied repeatedly.
-   The result of a C_simp_final simplification will not be simplified further.
-   For example, use C_simp_final when the RHS matches the LHS. *)
+text \<open>A simple proof method for rewriting Simpl programs under @{term ccorres_underlying}.\<close>
 
-named_theorems C_simp
+locale ccorres_rewrite_locale =
+  simpl_rewrite \<Gamma> "ccorres_underlying sr \<Gamma> r xf r' xf' P P' hs H"
+  for \<Gamma> sr r xf r' xf' P P' hs H
 
-context
-  (* for less typing and local com_eq syntax *)
-  fixes \<Gamma> :: "'b \<Rightarrow> ('a, 'b, 'c) com option"
-begin
+global_interpretation ccorres_rewrite: ccorres_rewrite_locale
+  by unfold_locales (auto simp: simpl_rewrite_base.com_eq_def semantic_equiv_def ceqv_def
+                          elim: ccorres_semantic_equivD2)
 
-definition
-  com_eq :: "('a, 'b, 'c) com \<Rightarrow> ('a, 'b, 'c) com \<Rightarrow> bool"
-where
-  "com_eq c c' \<equiv> \<forall>s s'. (\<Gamma> \<turnstile> \<langle>c,s\<rangle> \<Rightarrow> s') = (\<Gamma> \<turnstile> \<langle>c',s\<rangle> \<Rightarrow> s')"
+method ccorres_rewrite declares C_simp C_simp_pre C_simp_simps C_simp_throws
+  = ccorres_rewrite.simpl_rewrite
 
-(* local, in this context only *)
-notation com_eq (infix "\<sim>" 10)
+abbreviation "com_eq \<Gamma> \<equiv> ccorres_rewrite.com_eq \<Gamma> True"
+abbreviation "never_continues \<Gamma> \<equiv> ccorres_rewrite.never_continues \<Gamma> True"
 
-(* Slightly stronger than the existing semantic_equiv, which only talks about Normal s, not all s *)
-lemma com_eq_semantic_equiv:
-  "c \<sim> c' \<Longrightarrow> semantic_equiv \<Gamma> s s' c c'"
-  by (simp add: com_eq_def semantic_equiv_def ceqv_def)
+lemmas com_eq_def = ccorres_rewrite.com_eq_def
+lemmas never_continues_def = ccorres_rewrite.never_continues_def
 
-(* com_eq is an order *)
-lemma com_eq_refl:
-  "c \<sim> c"
-  by (simp add: com_eq_def)
+text \<open>Some CRefine proofs remove Collect_const from the @{method simp} set,
+      but we almost always want @{method ccorres_rewrite} to use it to simplify
+      trivial @{text IF} and @{text WHILE} conditions.\<close>
+declare Collect_const [C_simp_simps]
 
-lemma com_eq_sym:
-  "(c \<sim> c') = (c' \<sim> c)"
-  by (auto simp: com_eq_def)
+text \<open>Test that the @{command named_theorems} @{thm C_simp} still works in the
+      @{term ccorres_rewrite_locale} interpretation.\<close>
 
-lemma com_eq_trans:
-  "\<lbrakk> c \<sim> c'; c' \<sim> c'' \<rbrakk> \<Longrightarrow> c \<sim> c''"
-  by (auto simp: com_eq_def)
-
-(* com_eq permits rewriting under ccorres_underlying *)
-lemma ccorres_com_eqI:
-  "\<lbrakk> c \<sim> c'; ccorres_underlying sr \<Gamma> r xf r' xf' P P' hs H c' \<rbrakk> \<Longrightarrow>
-  ccorres_underlying sr \<Gamma> r xf r' xf' P P' hs H c"
-  by (erule ccorres_semantic_equivD2, erule com_eq_semantic_equiv)
-
-(* structural propagation rules *)
-lemma com_eq_Seq:
-  "\<lbrakk> c1 \<sim> c1'; c2 \<sim> c2' \<rbrakk> \<Longrightarrow> c1;;c2 \<sim> c1';;c2'"
-  unfolding com_eq_def
-  by (auto intro: exec.Seq elim!: exec_elim_cases)
-
-lemma com_eq_Cond:
-  "\<lbrakk> c1 \<sim> c1'; c2 \<sim> c2' \<rbrakk> \<Longrightarrow> Cond b c1 c2 \<sim> Cond b c1' c2'"
-  unfolding com_eq_def
-  by (auto intro: exec.CondTrue exec.CondFalse elim!: exec_elim_cases)
-
-lemma com_eq_While':
-  assumes eq: "c \<sim> c'"
-  assumes W: "\<Gamma> \<turnstile> \<langle>While b c,s\<rangle> \<Rightarrow> s'"
-  shows "\<Gamma> \<turnstile> \<langle>While b c',s\<rangle> \<Rightarrow> s'"
-  using W
-proof (induct "While b c" s s')
-  case WhileTrue
-  with eq show ?case unfolding com_eq_def by (auto elim: exec.WhileTrue)
-next
-  case WhileFalse
-  then show ?case by (rule exec.WhileFalse)
-qed auto
-
-lemma com_eq_While:
-  "c \<sim> c' \<Longrightarrow> While b c \<sim> While b c'"
-  by (subst com_eq_def)
-     (auto intro: com_eq_While' com_eq_While' [OF com_eq_sym [THEN iffD1]])
-
-(* the actual form of WHILE b DO c OD *)
-lemma com_eq_whileAnno:
-  "c \<sim> c' \<Longrightarrow> (whileAnno b I V c) \<sim> (whileAnno b I V c')"
-  by (clarsimp simp: whileAnno_def elim!: com_eq_While)
-
-lemma com_eq_Guard:
-  "c \<sim> c' \<Longrightarrow> Guard f b c \<sim> Guard f b c'"
-  unfolding com_eq_def
-  by (auto intro: exec.Guard exec.GuardFault elim!: exec_elim_cases)
-
-lemma com_eq_Catch:
-  "\<lbrakk> c \<sim> c'; h \<sim> h' \<rbrakk> \<Longrightarrow> Catch c h \<sim> Catch c' h'"
-  unfolding com_eq_def
-  by (auto intro: exec.CatchMiss exec.CatchMatch elim!: exec_elim_cases)
-
-lemmas ccorres_rewrite_splits =
-  com_eq_Seq com_eq_Cond com_eq_While com_eq_whileAnno com_eq_Guard com_eq_Catch
-
-(* Actual simplification rules *)
-
-lemma com_eq_Skip_Seq [C_simp]:
-  "c \<sim> c' \<Longrightarrow> Skip;;c \<sim> c'"
-  apply (clarsimp simp: com_eq_def)
-  apply (rule iffI)
-   apply (fastforce elim!: exec_elim_cases)
-  apply (case_tac s; (simp, (erule exec_elim_cases; simp)?))
-  apply (rule exec.Seq, rule exec.Skip, simp)
-  done
-
-lemma com_eq_Seq_Skip [C_simp]:
-  "c \<sim> c' \<Longrightarrow> c;;Skip \<sim> c'"
-  apply (clarsimp simp: com_eq_def)
-  apply (rule iffI)
-   apply (fastforce elim!: exec_elim_cases)
-  apply (case_tac s; (simp, (erule exec_elim_cases; simp)?))
-  apply (rule exec.Seq, simp)
-  apply (case_tac s'; (simp, (erule exec_elim_cases; simp)?))
-  apply (rule exec.Skip)
-  done
-
-lemma com_eq_Cond_empty [C_simp]:
-  "c \<sim> c' \<Longrightarrow> Cond {} c1 c \<sim> c'"
-  unfolding com_eq_def
-  by (clarsimp, case_tac s, auto intro: exec.CondFalse elim!: exec_elim_cases)
-
-lemma com_eq_Cond_UNIV [C_simp]:
-  "c \<sim> c' \<Longrightarrow> Cond UNIV c c2 \<sim> c'"
-  unfolding com_eq_def
-  by (clarsimp, case_tac s, auto intro: exec.CondTrue  elim!: exec_elim_cases)
-
-lemma exec_Cond_cases:
-  "\<lbrakk>s \<in> b \<Longrightarrow> \<Gamma>\<turnstile> \<langle>c\<^sub>1,Normal s\<rangle> \<Rightarrow> t; s \<notin> b \<Longrightarrow> \<Gamma>\<turnstile> \<langle>c\<^sub>2,Normal s\<rangle> \<Rightarrow> t\<rbrakk> \<Longrightarrow>
-  \<Gamma>\<turnstile> \<langle>Cond b c\<^sub>1 c\<^sub>2,Normal s\<rangle> \<Rightarrow> t"
-  by (cases "s \<in> b") (auto intro: exec.CondTrue exec.CondFalse)
-
-lemma com_eq_Cond_both [C_simp]:
-  "c \<sim> c' \<Longrightarrow> Cond b c c \<sim> c'"
-  unfolding com_eq_def
-  by (clarsimp, case_tac s, auto intro: exec_Cond_cases elim!: exec_elim_cases)
-
-lemma com_eq_If_False [C_simp]:
-  "c \<sim> c' \<Longrightarrow> IF False THEN c1 ELSE c FI \<sim> c'"
-  by (simp add: com_eq_Cond_empty)
-
-lemma com_eq_If_True [C_simp]:
-  "c \<sim> c' \<Longrightarrow> IF True THEN c ELSE c2 FI \<sim> c'"
-  by (simp add: com_eq_Cond_UNIV)
-
-lemma com_eq_While_empty [C_simp]:
-  "While {} c \<sim> Skip"
-  unfolding com_eq_def
-  by (auto intro: exec.WhileFalse exec.Skip elim!: exec_elim_cases)
-
-lemma com_eq_While_FALSE [C_simp]:
-  "WHILE False INV P DO c OD \<sim> Skip"
-  by (simp add: com_eq_While_empty whileAnno_def)
-
-lemma com_eq_Guard_UNIV [C_simp]:
-  "c \<sim> c' \<Longrightarrow> Guard f UNIV c \<sim> c'"
-  unfolding com_eq_def
-  by (clarsimp, case_tac s, auto intro: exec.Guard elim!: exec_elim_cases)
-
-lemma com_eq_Guard_True [C_simp]:
-  "c \<sim> c' \<Longrightarrow> Guard f \<lbrace>True\<rbrace> c \<sim> c'"
-  by (clarsimp simp: com_eq_Guard_UNIV)
-
-lemma com_eq_Guard_empty [C_simp]:
-  "Guard f {} c \<sim> Guard f {} Skip"
-  unfolding com_eq_def
-  by (clarsimp, case_tac s, auto intro: exec.GuardFault elim!: exec_elim_cases)
-
-lemma com_eq_Guard_False [C_simp]:
-  "Guard f \<lbrace>False\<rbrace> c \<sim> Guard f {} Skip"
-  by (clarsimp simp: com_eq_Guard_empty)
-
-lemma com_eq_Catch_Skip [C_simp]:
-  "Catch Skip c \<sim> Skip"
-  unfolding com_eq_def
-  by (auto intro: exec.CatchMiss exec.Skip elim!: exec_elim_cases)
-
-lemma com_eq_Catch_Throw [C_simp]:
-  "c \<sim> c' \<Longrightarrow> Catch Throw c \<sim> c'"
-  unfolding com_eq_def
-  by (clarsimp, case_tac s, auto intro: exec.CatchMatch exec.Throw elim!: exec_elim_cases)
-
-lemma com_eq_Throw [C_simp]:
-  "Throw;; c \<sim> Throw"
-  unfolding com_eq_def
-  by (auto intro: exec.Throw exec.Seq elim!: exec_elim_cases)
-
-end
-
-
-(* First introduces com_eq goal (rule cccorres_com_eqI), then breaks the term into
-   its component parts (ccorres_rewrite_decompose), and finally reassembles,
-   applying simplification rules whenever possible, and otherwise applying reflexivity.
-
-   At every decomposition or simplification step, we first apply a transitivity rule,
-   to ensure we can continue simplifying each subterm until no more simplifications
-   are possible, before applying reflexivity to reassemble the enclosing term.
-
-   Limited to unconditional rewrite rules. Purpose is not to provide a real rewriting engine,
-   just to get rid of annoying Skip and Cond {} bits that come from config options or macros.
-*)
-
-method ccorres_rewrite_decompose =
-  (rule com_eq_trans, (rule ccorres_rewrite_splits; ccorres_rewrite_decompose)?)
-
-method ccorres_rewrite_recombine declares C_simp =
-  determ \<open>rule C_simp com_eq_refl\<close>
-
-method ccorres_rewrite declares C_simp =
-  changed \<open>rule ccorres_com_eqI, ccorres_rewrite_decompose, ccorres_rewrite_recombine+\<close>
-
-(* Example *)
 lemma
   assumes c3: "com_eq \<Gamma> c3 c"
   assumes c: "com_eq \<Gamma> (c;;c) c"
@@ -231,66 +50,13 @@ lemma
                             (c;; Guard f UNIV (IF X THEN c ELSE c FI);; Cond {} Skip (Skip;;c2);;
                              Skip;;
                              (IF False THEN Skip ELSE SKIP;; TRY THROW CATCH c3 END FI;; SKIP))"
-  apply ccorres_rewrite              (* c;; c;; c2;; c3 *)
+  apply ccorres_rewrite
   apply (match conclusion in "ccorres_underlying sr \<Gamma> r xf r' xf' P P' hs H (c;;c;;c2;;c3)" \<Rightarrow> \<open>-\<close>)
-  apply (ccorres_rewrite C_simp: c3) (* c;; c;; c2;; c *)
+  apply (ccorres_rewrite C_simp: c3)
   apply (match conclusion in "ccorres_underlying sr \<Gamma> r xf r' xf' P P' hs H (c;;c;;c2;;c)" \<Rightarrow> \<open>-\<close>)
-  apply (ccorres_rewrite C_simp: c)  (* c;; c2;; c *)
+  apply (ccorres_rewrite C_simp: c)
   apply (match conclusion in "ccorres_underlying sr \<Gamma> r xf r' xf' P P' hs H (c;;c2;;c)" \<Rightarrow> \<open>-\<close>)
-  apply (fails \<open>ccorres_rewrite\<close>)    (* fails if nothing changes *)
-  oops
-
-(* Test for WHILE (whileAnno) case *)
-lemma "ccorres_underlying sr \<Gamma> r xf r' xf' P P' hs H
-        (WHILE b DO Guard f g c;; IF False THEN c2 FI OD;; SKIP)"
-  apply ccorres_rewrite
-  apply (match conclusion in "ccorres_underlying sr \<Gamma> r xf r' xf' P P' hs H
-                                (WHILE b DO Guard f g c OD)" \<Rightarrow> \<open>-\<close>)
-  oops
-
-(* Test that simplification works down all branches of the term. *)
-lemma "ccorres_underlying sr \<Gamma> r xf r' xf' P P' hs H
-           (IF b THEN
-              (SKIP ;; c) ;; (SKIP ;; IF True THEN SKIP ELSE c FI)
-            ELSE
-              (SKIP ;; SKIP) ;; (Guard f UNIV c ;; SKIP)
-            FI)"
-  apply ccorres_rewrite
-  apply (match conclusion in "ccorres_underlying sr \<Gamma> r xf r' xf' P P' hs H c" \<Rightarrow> \<open>-\<close>)
-  oops
-
-(* Test that complex simplification rules work. *)
-context begin
-
-private lemma com_eq_Cond_redundant:
-  "com_eq \<Gamma> (IF b THEN c1 ELSE IF b THEN c2 ELSE c3 FI FI) (IF b THEN c1 ELSE c3 FI)"
-  unfolding com_eq_def
-  by (auto intro: exec.CondTrue exec.CondFalse elim!: exec_elim_cases)
-
-private lemma "ccorres_underlying sr \<Gamma> r xf r' xf' P P' hs H
-                (SKIP ;;
-                 IF b THEN
-                   (SKIP ;; c1) ;; (SKIP ;; SKIP)
-                 ELSE
-                   IF b THEN
-                     IF b1 THEN c2 ELSE c2 FI
-                   ELSE
-                     WHILE False DO c4 OD ;; (c3 ;; SKIP)
-                   FI
-                 FI)"
-  apply (ccorres_rewrite C_simp: com_eq_Cond_redundant)
-  apply (match conclusion in "ccorres_underlying sr \<Gamma> r xf r' xf' P P' hs H
-                                (IF b THEN c1 ELSE c3 FI)" \<Rightarrow> \<open>-\<close>)
-  oops
-
-end
-
-(* Test False guard avoids looping. *)
-lemma "ccorres_underlying sr \<Gamma> r xf r' xf' P P' hs H
-        (SKIP ;; Guard f {} (IF b THEN c ELSE c FI) ;; SKIP)"
-  apply ccorres_rewrite
-  apply (match conclusion in "ccorres_underlying sr \<Gamma> r xf r' xf' P P' hs H
-                                (Guard f {} SKIP)" \<Rightarrow> \<open>-\<close>)
+  apply (fails \<open>ccorres_rewrite\<close>)
   oops
 
 end
